Some progress on modeling data structures
Got stuck on dealing with type indices; couldn't write down a strong
update on well-typed state of the form [forall T, IORef T -> T] since
the indices [T & IORef T] would need decidable equality and I'm not sure
about assuming that. In theory it's fine, but we can't actually compare
heterogeneous IORefs in Haskell (the only facility I know of to do this
is Data.Typeable, and IORefs don't implement Typeable). This is a
strange issue since I'm having trouble giving a _model_ of IORefs, not
assuming pure functions to use them.

Solved this problem by modeling IORefs using type codes. Reads are an
Err in the semantics if the "guessed" type isn't correct.

src/Database/DataStructures.v
@@ -1,12 +1,44 @@
 From RecoveryRefinement Require Import Helpers.MachinePrimitives.
 From RecoveryRefinement Require Import Spec.Proc.
 From RecoveryRefinement Require Import Spec.SumProc.
+From RecoveryRefinement Require Import Helpers.RelationAlgebra.
+
+From RecordUpdate Require Import RecordSet.
+Import ApplicativeNotations.
+
+From Classes Require Import EqualDec.
+From Coq Require Import Program.Equality.
+Import EqNotations.
 
 Set Implicit Arguments.
 
-Axiom Array : Type -> Type.
-Axiom IORef : Type -> Type.
+Module ty.
+  Inductive t : Type :=
+  | Fd
+  | uint64
+  | ByteString
+  .
+End ty.
 
+Definition ty := ty.t.
+
+Coercion Ty (T:ty) : Type :=
+  match T with
+  | ty.Fd => Fd
+  | ty.uint64 => uint64
+  | ty.ByteString => ByteString
+  end.
+
+Axiom IORef_ : Type.
+Axiom ioref_eqdec : EqualDec IORef_.
+Existing Instance ioref_eqdec.
+
+Definition IORef (T:ty) := IORef_.
+
+(* TODO: fix Arrays to be same as IORef *)
+Axiom Array : Type -> Type.
+
+(* TODO: fix Vars to be same as IORef *)
 Inductive LogVar : Type -> Type :=
 | File : LogVar Fd
 .
@@ -15,6 +47,27 @@ Inductive Var : Type -> Type :=
 | Log : forall T, LogVar T -> Var T
 .
 
+Instance var_eqdec T : EqualDec (Var T).
+Proof.
+  hnf; intros.
+  destruct x, y.
+  - dependent destruction l; dependent destruction l0; auto.
+Defined.
+
+(* hetereogeneous equality of a type family *)
+Class HEqDec A (F: A -> Type) :=
+  heq_dec : forall a1 a2 (x: F a1) (y: F a2),
+    {H & (rew H in x) = y} + {forall H, (rew H in x) <> y}.
+
+Definition var_eq T1 T2 (x: Var T1) (y: Var T2) :
+  {H & (rew H in x) = y} + {forall H, (rew H in x) <> y}.
+Proof.
+  destruct x, y.
+  - dependent destruction l; dependent destruction l0.
+    left.
+    exists eq_refl; auto.
+Defined.
+
 Module Data.
   Inductive Op : Type -> Type :=
   (* generic variable operations *)
@@ -22,7 +75,7 @@ Module Data.
   | SetVar : forall T, Var T -> T -> Op T
 
   (* arbitrary references *)
-  | NewIORef : forall T, T -> Op (IORef T)
+  | NewIORef : forall (T:ty), T -> Op (IORef T)
   | ReadIORef : forall T, IORef T -> Op T
   | WriteIORef : forall T, IORef T -> T -> Op unit
 
@@ -38,12 +91,12 @@ Module Data.
   Definition get Op' {i:Injectable Op Op'} T (var: Var T) : proc Op' T :=
     Call (inject (GetVar var)).
 
-  Definition set Op' {i:Injectable Op Op'} T (var: Var T) (v: T) : proc Op' T :=
+  Definition set_var Op' {i:Injectable Op Op'} T (var: Var T) (v: T) : proc Op' T :=
     Call (inject (SetVar var v)).
 
   Definition newIORef Op' {i:Injectable Op Op'}
-             T (v:T) : proc Op' (IORef T) :=
-    Call (inject (NewIORef v)).
+             (T:ty) (v:T) : proc Op' (IORef T) :=
+    Call (inject (NewIORef T v)).
 
   Definition readIORef Op' {i:Injectable Op Op'}
              T (ref:IORef T) : proc Op' T :=
@@ -62,6 +115,48 @@ Module Data.
 
   Definition arrayAppend Op' {i:Injectable Op Op'} T (a: Array T) (v:T) : proc Op' unit :=
     Call (inject (ArrayAppend a v)).
+
+  Record State : Type :=
+    mkState { iorefs: IORef_ -> option {T:ty & T};
+              (* TODO: similar model for variables (except complete map) and
+              arrays *) }.
+
+  Instance _eta : Settable _ :=
+    mkSettable (constructor mkState <*> iorefs)%set.
+
+  Definition upd_iorefs T (v: IORef T) (x: T)
+             (f:IORef_ -> option {T:ty & T}) : IORef_ -> option {T:ty & T}
+    := fun r => if equal r v then Some (existT T x) else f r.
+
+  Definition get_ioref T (v: IORef T)
+             (f:IORef_ -> option {T:ty & T}) : option T :=
+    match f v with
+    | Some (existT T' x) =>
+      match equal T' T with
+      | left H => Some (rew H in x)
+      | right _ => None
+      end
+    | None => None
+    end.
+
+  Import RelationNotations.
+
+  Definition step T (op:Op T) : relation State State T :=
+    match op in Op T return relation State State T with
+    (* | GetVar v => reads (fun s => vars s v) *)
+    (* | SetVar v x => puts (set vars (fupd v x)) *)
+    | NewIORef _ x =>
+      r <- such_that (fun s r => s.(iorefs) r = None);
+        _ <- puts (set iorefs (upd_iorefs r x));
+        pure r
+    | WriteIORef v x =>
+      _ <- readSome (fun s => s.(iorefs) v);
+        puts (set iorefs (upd_iorefs v x))
+    | ReadIORef v =>
+      readSome (fun s => get_ioref v s.(iorefs))
+    | _ => error
+    end.
+
 End Data.
 
 (* TODO: we should be able to make this pattern more convenient, but for now
